theories/L2k_noCnstrParams/toplevel.v
@@ -1,13 +1,54 @@
 Require Import L2k.compile.
 Require Import L2k.wcbvEval.
 Require Import L2k.term.
-Require Import L2k.stripEvalCommute.
 Require Import Common.Common Common.compM Common.Pipeline_utils.
-Require Import L1g.toplevel.
 From ExtLib Require Import Monads.
 
+
+Require Import Common.Common Common.classes Common.Pipeline_utils Common.compM.
+From ExtLib Require Import Monads.
+From MetaCoq.Template Require Import utils Typing.
 Import MonadNotation.
 
+(* 
+Definition erase_PCUIC : CertiCoqTrans Ast.Env.program (global_context * term) :=
+  fun src =>
+    debug_msg "Translating from Template to Lbox" ;;
+    (LiftErrorCertiCoqTrans "Lbox" L1g.compile.erase src).
+
+(* Expose the top-level transformation function *)
+Definition compile_L1g : CertiCoqTrans (global_context * term) (Program Term) :=
+  fun src =>
+    debug_msg "Translating from Lbox to L1" ;;
+    (LiftCertiCoqTrans "L1g" L1g.compile.program_Program src).
+
+
+
+
+#[global] Instance L1g_Lang : Lang (Program Term) :=
+  { Value := Term;
+    TermWf := fun P => match P with
+                      mkPgm trm env => WFapp trm /\ program.WFaEnv env
+                    end;
+    BigStep := fun s sv => WcbvEval (env s) (main s) sv
+  }.
+ *)
+
+ Definition wf_program (p : Ast.Env.program) := 
+  ∥ ∑ T, @Typing.typing 
+    config.extraction_checker_flags
+    (Ast.Env.empty_ext p.1)
+    [] p.2 T ∥.
+
+Definition template_bigstep (p : Ast.Env.program) (v : Ast.term) : Prop :=
+  ∥ Template.WcbvEval.eval p.1 p.2 v ∥.
+ 
+ #[export] Instance Template_Lang : Lang Ast.Env.program :=
+  { Value := Ast.term;
+    TermWf := wf_program ;
+    BigStep := template_bigstep }. 
+
+Import MonadNotation.
 
 Instance L2k_Lang : Lang (Program L2k.compile.Term) :=
   { Value := Term;
@@ -15,10 +56,480 @@ Instance L2k_Lang : Lang (Program L2k.compile.Term) :=
     BigStep := fun s sv => WcbvEval (env s) (main s) sv
   }.
 
-
 Definition compile_L2k
-  : CertiCoqTrans (Program L1g.compile.Term) (Program L2k.compile.Term) :=
+  : CertiCoqTrans (Ast.Env.program) (Program L2k.compile.Term) :=
   fun src =>
     debug_msg "Translating from L1g to L1k" ;;
-    (LiftCertiCoqTrans "L2k" stripProgram src).
+    (LiftCertiCoqTrans "L2k" compile_program src).
 
+Goal compile_program = compile_program.
+Proof.
+  unfold compile_program.
+  unfold Erasure.erase_program.
+  unfold Erasure.expand_program.
+  unfold Erasure.erasure_pipeline.
+
+
+1/1
+(fun p : Ast.Env.program =>
+ {|
+   main :=
+     compile
+       (Erasure.Transform.run
+          (Erasure.Transform.compose
+             (Erasure.Transform.compose
+                (Erasure.Transform.compose
+                   (Erasure.Transform.compose
+                      Erasure.template_to_pcuic_transform
+                      Erasure.pcuic_expand_lets_transform
+                      (fun (p0 : Erasure.pcuic_program)
+                         (H : Erasure.Transform.post
+                                Erasure.template_to_pcuic_transform p0) =>
+                       Erasure.erasure_pipeline_obligation_1 p0 H))
+                   Erasure.erase_transform
+                   (fun (p0 : Erasure.pcuic_program)
+                      (H : Erasure.Transform.post
+                             (Erasure.Transform.compose
+                                Erasure.template_to_pcuic_transform
+                                Erasure.pcuic_expand_lets_transform
+                                (fun (p1 : Erasure.pcuic_program)
+                                   (H : Erasure.Transform.post
+                                          Erasure.template_to_pcuic_transform
+                                          p1) =>
+                                 Erasure.erasure_pipeline_obligation_1 p1 H))
+                             p0) =>
+                    Erasure.erasure_pipeline_obligation_2 p0 H))
+                (Erasure.remove_params_optimization
+                   EWcbvEval.default_wcbv_flags)
+                (fun (p0 : Erasure.eprogram_env)
+                   (_ : Erasure.Transform.post
+                          (Erasure.Transform.compose
+                             (Erasure.Transform.compose
+                                Erasure.template_to_pcuic_transform
+                                Erasure.pcuic_expand_lets_transform
+                                (fun (p1 : Erasure.pcuic_program)
+                                   (H : Erasure.Transform.post
+                                          Erasure.template_to_pcuic_transform
+                                          p1) =>
+                                 Erasure.erasure_pipeline_obligation_1 p1 H))
+                             Erasure.erase_transform
+                             (fun (p1 : Erasure.pcuic_program)
+                                (H : Erasure.Transform.post
+                                       (Erasure.Transform.compose
+                                          Erasure.template_to_pcuic_transform
+                                          Erasure.pcuic_expand_lets_transform
+                                          (fun (p2 : Erasure.pcuic_program)
+                                             (H : 
+                                              Erasure.Transform.post
+                                                Erasure.template_to_pcuic_transform
+                                                p2) =>
+                                           Erasure.erasure_pipeline_obligation_1
+                                             p2 H)) p1) =>
+                              Erasure.erasure_pipeline_obligation_2 p1 H)) p0)
+                 => Erasure.erasure_pipeline_obligation_3 p0))
+             Erasure.optimize_prop_discr_optimization
+             (fun (p0 : Erasure.eprogram)
+                (H : Erasure.Transform.post
+                       (Erasure.Transform.compose
+                          (Erasure.Transform.compose
+                             (Erasure.Transform.compose
+                                Erasure.template_to_pcuic_transform
+                                Erasure.pcuic_expand_lets_transform
+                                (fun (p1 : Erasure.pcuic_program)
+                                   (H : Erasure.Transform.post
+                                          Erasure.template_to_pcuic_transform
+                                          p1) =>
+                                 Erasure.erasure_pipeline_obligation_1 p1 H))
+                             Erasure.erase_transform
+                             (fun (p1 : Erasure.pcuic_program)
+                                (H : Erasure.Transform.post
+                                       (Erasure.Transform.compose
+                                          Erasure.template_to_pcuic_transform
+                                          Erasure.pcuic_expand_lets_transform
+                                          (fun (p2 : Erasure.pcuic_program)
+                                             (H : 
+                                              Erasure.Transform.post
+                                                Erasure.template_to_pcuic_transform
+                                                p2) =>
+                                           Erasure.erasure_pipeline_obligation_1
+                                             p2 H)) p1) =>
+                              Erasure.erasure_pipeline_obligation_2 p1 H))
+                          (Erasure.remove_params_optimization
+                             EWcbvEval.default_wcbv_flags)
+                          (fun (p1 : Erasure.eprogram_env)
+                             (_ : Erasure.Transform.post
+                                    (Erasure.Transform.compose
+                                       (Erasure.Transform.compose
+                                          Erasure.template_to_pcuic_transform
+                                          Erasure.pcuic_expand_lets_transform
+                                          (fun (p2 : Erasure.pcuic_program)
+                                             (H : 
+                                              Erasure.Transform.post
+                                                Erasure.template_to_pcuic_transform
+                                                p2) =>
+                                           Erasure.erasure_pipeline_obligation_1
+                                             p2 H)) Erasure.erase_transform
+                                       (fun (p2 : Erasure.pcuic_program)
+                                          (H : Erasure.Transform.post
+                                                 (Erasure.Transform.compose
+                                                 Erasure.template_to_pcuic_transform
+                                                 Erasure.pcuic_expand_lets_transform
+                                                 (fun
+                                                 (p3 : Erasure.pcuic_program)
+                                                 (H : 
+                                                 Erasure.Transform.post
+                                                 Erasure.template_to_pcuic_transform
+                                                 p3) =>
+                                                 Erasure.erasure_pipeline_obligation_1
+                                                 p3 H)) p2) =>
+                                        Erasure.erasure_pipeline_obligation_2
+                                          p2 H)) p1) =>
+                           Erasure.erasure_pipeline_obligation_3 p1)) p0) =>
+              Erasure.erasure_pipeline_obligation_4 p0 H))
+          (Erasure.expand_program p) (todo "wf_env and welltyped term")).2;
+   env :=
+     compile_ctx
+       (Erasure.Transform.run
+          (Erasure.Transform.compose
+             (Erasure.Transform.compose
+                (Erasure.Transform.compose
+                   (Erasure.Transform.compose
+                      Erasure.template_to_pcuic_transform
+                      Erasure.pcuic_expand_lets_transform
+                      (fun (p0 : Erasure.pcuic_program)
+                         (H : Erasure.Transform.post
+                                Erasure.template_to_pcuic_transform p0) =>
+                       Erasure.erasure_pipeline_obligation_1 p0 H))
+                   Erasure.erase_transform
+                   (fun (p0 : Erasure.pcuic_program)
+                      (H : Erasure.Transform.post
+                             (Erasure.Transform.compose
+                                Erasure.template_to_pcuic_transform
+                                Erasure.pcuic_expand_lets_transform
+                                (fun (p1 : Erasure.pcuic_program)
+                                   (H : Erasure.Transform.post
+                                          Erasure.template_to_pcuic_transform
+                                          p1) =>
+                                 Erasure.erasure_pipeline_obligation_1 p1 H))
+                             p0) =>
+                    Erasure.erasure_pipeline_obligation_2 p0 H))
+                (Erasure.remove_params_optimization
+                   EWcbvEval.default_wcbv_flags)
+                (fun (p0 : Erasure.eprogram_env)
+                   (_ : Erasure.Transform.post
+                          (Erasure.Transform.compose
+                             (Erasure.Transform.compose
+                                Erasure.template_to_pcuic_transform
+                                Erasure.pcuic_expand_lets_transform
+                                (fun (p1 : Erasure.pcuic_program)
+                                   (H : Erasure.Transform.post
+                                          Erasure.template_to_pcuic_transform
+                                          p1) =>
+                                 Erasure.erasure_pipeline_obligation_1 p1 H))
+                             Erasure.erase_transform
+                             (fun (p1 : Erasure.pcuic_program)
+                                (H : Erasure.Transform.post
+                                       (Erasure.Transform.compose
+                                          Erasure.template_to_pcuic_transform
+                                          Erasure.pcuic_expand_lets_transform
+                                          (fun (p2 : Erasure.pcuic_program)
+                                             (H : 
+                                              Erasure.Transform.post
+                                                Erasure.template_to_pcuic_transform
+                                                p2) =>
+                                           Erasure.erasure_pipeline_obligation_1
+                                             p2 H)) p1) =>
+                              Erasure.erasure_pipeline_obligation_2 p1 H)) p0)
+                 => Erasure.erasure_pipeline_obligation_3 p0))
+             Erasure.optimize_prop_discr_optimization
+             (fun (p0 : Erasure.eprogram)
+                (H : Erasure.Transform.post
+                       (Erasure.Transform.compose
+                          (Erasure.Transform.compose
+                             (Erasure.Transform.compose
+                                Erasure.template_to_pcuic_transform
+                                Erasure.pcuic_expand_lets_transform
+                                (fun (p1 : Erasure.pcuic_program)
+                                   (H : Erasure.Transform.post
+                                          Erasure.template_to_pcuic_transform
+                                          p1) =>
+                                 Erasure.erasure_pipeline_obligation_1 p1 H))
+                             Erasure.erase_transform
+                             (fun (p1 : Erasure.pcuic_program)
+                                (H : Erasure.Transform.post
+                                       (Erasure.Transform.compose
+                                          Erasure.template_to_pcuic_transform
+                                          Erasure.pcuic_expand_lets_transform
+                                          (fun (p2 : Erasure.pcuic_program)
+                                             (H : 
+                                              Erasure.Transform.post
+                                                Erasure.template_to_pcuic_transform
+                                                p2) =>
+                                           Erasure.erasure_pipeline_obligation_1
+                                             p2 H)) p1) =>
+                              Erasure.erasure_pipeline_obligation_2 p1 H))
+                          (Erasure.remove_params_optimization
+                             EWcbvEval.default_wcbv_flags)
+                          (fun (p1 : Erasure.eprogram_env)
+                             (_ : Erasure.Transform.post
+                                    (Erasure.Transform.compose
+                                       (Erasure.Transform.compose
+                                          Erasure.template_to_pcuic_transform
+                                          Erasure.pcuic_expand_lets_transform
+                                          (fun (p2 : Erasure.pcuic_program)
+                                             (H : 
+                                              Erasure.Transform.post
+                                                Erasure.template_to_pcuic_transform
+                                                p2) =>
+                                           Erasure.erasure_pipeline_obligation_1
+                                             p2 H)) Erasure.erase_transform
+                                       (fun (p2 : Erasure.pcuic_program)
+                                          (H : Erasure.Transform.post
+                                                 (Erasure.Transform.compose
+                                                 Erasure.template_to_pcuic_transform
+                                                 Erasure.pcuic_expand_lets_transform
+                                                 (fun
+                                                 (p3 : Erasure.pcuic_program)
+                                                 (H : 
+                                                 Erasure.Transform.post
+                                                 Erasure.template_to_pcuic_transform
+                                                 p3) =>
+                                                 Erasure.erasure_pipeline_obligation_1
+                                                 p3 H)) p2) =>
+                                        Erasure.erasure_pipeline_obligation_2
+                                          p2 H)) p1) =>
+                           Erasure.erasure_pipeline_obligation_3 p1)) p0) =>
+              Erasure.erasure_pipeline_obligation_4 p0 H))
+          (Erasure.expand_program p) (todo "wf_env and welltyped term")).1
+ |}) =
+(fun p : Ast.Env.program =>
+ {|
+   main :=
+     compile
+       (Erasure.Transform.run
+          (Erasure.Transform.compose
+             (Erasure.Transform.compose
+                (Erasure.Transform.compose
+                   (Erasure.Transform.compose
+                      Erasure.template_to_pcuic_transform
+                      Erasure.pcuic_expand_lets_transform
+                      (fun (p0 : Erasure.pcuic_program)
+                         (H : Erasure.Transform.post
+                                Erasure.template_to_pcuic_transform p0) =>
+                       Erasure.erasure_pipeline_obligation_1 p0 H))
+                   Erasure.erase_transform
+                   (fun (p0 : Erasure.pcuic_program)
+                      (H : Erasure.Transform.post
+                             (Erasure.Transform.compose
+                                Erasure.template_to_pcuic_transform
+                                Erasure.pcuic_expand_lets_transform
+                                (fun (p1 : Erasure.pcuic_program)
+                                   (H : Erasure.Transform.post
+                                          Erasure.template_to_pcuic_transform
+                                          p1) =>
+                                 Erasure.erasure_pipeline_obligation_1 p1 H))
+                             p0) =>
+                    Erasure.erasure_pipeline_obligation_2 p0 H))
+                (Erasure.remove_params_optimization
+                   EWcbvEval.default_wcbv_flags)
+                (fun (p0 : Erasure.eprogram_env)
+                   (_ : Erasure.Transform.post
+                          (Erasure.Transform.compose
+                             (Erasure.Transform.compose
+                                Erasure.template_to_pcuic_transform
+                                Erasure.pcuic_expand_lets_transform
+                                (fun (p1 : Erasure.pcuic_program)
+                                   (H : Erasure.Transform.post
+                                          Erasure.template_to_pcuic_transform
+                                          p1) =>
+                                 Erasure.erasure_pipeline_obligation_1 p1 H))
+                             Erasure.erase_transform
+                             (fun (p1 : Erasure.pcuic_program)
+                                (H : Erasure.Transform.post
+                                       (Erasure.Transform.compose
+                                          Erasure.template_to_pcuic_transform
+                                          Erasure.pcuic_expand_lets_transform
+                                          (fun (p2 : Erasure.pcuic_program)
+                                             (H : 
+                                              Erasure.Transform.post
+                                                Erasure.template_to_pcuic_transform
+                                                p2) =>
+                                           Erasure.erasure_pipeline_obligation_1
+                                             p2 H)) p1) =>
+                              Erasure.erasure_pipeline_obligation_2 p1 H)) p0)
+                 => Erasure.erasure_pipeline_obligation_3 p0))
+             Erasure.optimize_prop_discr_optimization
+             (fun (p0 : Erasure.eprogram)
+                (H : Erasure.Transform.post
+                       (Erasure.Transform.compose
+                          (Erasure.Transform.compose
+                             (Erasure.Transform.compose
+                                Erasure.template_to_pcuic_transform
+                                Erasure.pcuic_expand_lets_transform
+                                (fun (p1 : Erasure.pcuic_program)
+                                   (H : Erasure.Transform.post
+                                          Erasure.template_to_pcuic_transform
+                                          p1) =>
+                                 Erasure.erasure_pipeline_obligation_1 p1 H))
+                             Erasure.erase_transform
+                             (fun (p1 : Erasure.pcuic_program)
+                                (H : Erasure.Transform.post
+                                       (Erasure.Transform.compose
+                                          Erasure.template_to_pcuic_transform
+                                          Erasure.pcuic_expand_lets_transform
+                                          (fun (p2 : Erasure.pcuic_program)
+                                             (H : 
+                                              Erasure.Transform.post
+                                                Erasure.template_to_pcuic_transform
+                                                p2) =>
+                                           Erasure.erasure_pipeline_obligation_1
+                                             p2 H)) p1) =>
+                              Erasure.erasure_pipeline_obligation_2 p1 H))
+                          (Erasure.remove_params_optimization
+                             EWcbvEval.default_wcbv_flags)
+                          (fun (p1 : Erasure.eprogram_env)
+                             (_ : Erasure.Transform.post
+                                    (Erasure.Transform.compose
+                                       (Erasure.Transform.compose
+                                          Erasure.template_to_pcuic_transform
+                                          Erasure.pcuic_expand_lets_transform
+                                          (fun (p2 : Erasure.pcuic_program)
+                                             (H : 
+                                              Erasure.Transform.post
+                                                Erasure.template_to_pcuic_transform
+                                                p2) =>
+                                           Erasure.erasure_pipeline_obligation_1
+                                             p2 H)) Erasure.erase_transform
+                                       (fun (p2 : Erasure.pcuic_program)
+                                          (H : Erasure.Transform.post
+                                                 (Erasure.Transform.compose
+                                                 Erasure.template_to_pcuic_transform
+                                                 Erasure.pcuic_expand_lets_transform
+                                                 (fun
+                                                 (p3 : Erasure.pcuic_program)
+                                                 (H : 
+                                                 Erasure.Transform.post
+                                                 Erasure.template_to_pcuic_transform
+                                                 p3) =>
+                                                 Erasure.erasure_pipeline_obligation_1
+                                                 p3 H)) p2) =>
+                                        Erasure.erasure_pipeline_obligation_2
+                                          p2 H)) p1) =>
+                           Erasure.erasure_pipeline_obligation_3 p1)) p0) =>
+              Erasure.erasure_pipeline_obligation_4 p0 H))
+          (Erasure.expand_program p) (todo "wf_env and welltyped term")).2;
+   env :=
+     compile_ctx
+       (Erasure.Transform.run
+          (Erasure.Transform.compose
+             (Erasure.Transform.compose
+                (Erasure.Transform.compose
+                   (Erasure.Transform.compose
+                      Erasure.template_to_pcuic_transform
+                      Erasure.pcuic_expand_lets_transform
+                      (fun (p0 : Erasure.pcuic_program)
+                         (H : Erasure.Transform.post
+                                Erasure.template_to_pcuic_transform p0) =>
+                       Erasure.erasure_pipeline_obligation_1 p0 H))
+                   Erasure.erase_transform
+                   (fun (p0 : Erasure.pcuic_program)
+                      (H : Erasure.Transform.post
+                             (Erasure.Transform.compose
+                                Erasure.template_to_pcuic_transform
+                                Erasure.pcuic_expand_lets_transform
+                                (fun (p1 : Erasure.pcuic_program)
+                                   (H : Erasure.Transform.post
+                                          Erasure.template_to_pcuic_transform
+                                          p1) =>
+                                 Erasure.erasure_pipeline_obligation_1 p1 H))
+                             p0) =>
+                    Erasure.erasure_pipeline_obligation_2 p0 H))
+                (Erasure.remove_params_optimization
+                   EWcbvEval.default_wcbv_flags)
+                (fun (p0 : Erasure.eprogram_env)
+                   (_ : Erasure.Transform.post
+                          (Erasure.Transform.compose
+                             (Erasure.Transform.compose
+                                Erasure.template_to_pcuic_transform
+                                Erasure.pcuic_expand_lets_transform
+                                (fun (p1 : Erasure.pcuic_program)
+                                   (H : Erasure.Transform.post
+                                          Erasure.template_to_pcuic_transform
+                                          p1) =>
+                                 Erasure.erasure_pipeline_obligation_1 p1 H))
+                             Erasure.erase_transform
+                             (fun (p1 : Erasure.pcuic_program)
+                                (H : Erasure.Transform.post
+                                       (Erasure.Transform.compose
+                                          Erasure.template_to_pcuic_transform
+                                          Erasure.pcuic_expand_lets_transform
+                                          (fun (p2 : Erasure.pcuic_program)
+                                             (H : 
+                                              Erasure.Transform.post
+                                                Erasure.template_to_pcuic_transform
+                                                p2) =>
+                                           Erasure.erasure_pipeline_obligation_1
+                                             p2 H)) p1) =>
+                              Erasure.erasure_pipeline_obligation_2 p1 H)) p0)
+                 => Erasure.erasure_pipeline_obligation_3 p0))
+             Erasure.optimize_prop_discr_optimization
+             (fun (p0 : Erasure.eprogram)
+                (H : Erasure.Transform.post
+                       (Erasure.Transform.compose
+                          (Erasure.Transform.compose
+                             (Erasure.Transform.compose
+                                Erasure.template_to_pcuic_transform
+                                Erasure.pcuic_expand_lets_transform
+                                (fun (p1 : Erasure.pcuic_program)
+                                   (H : Erasure.Transform.post
+                                          Erasure.template_to_pcuic_transform
+                                          p1) =>
+                                 Erasure.erasure_pipeline_obligation_1 p1 H))
+                             Erasure.erase_transform
+                             (fun (p1 : Erasure.pcuic_program)
+                                (H : Erasure.Transform.post
+                                       (Erasure.Transform.compose
+                                          Erasure.template_to_pcuic_transform
+                                          Erasure.pcuic_expand_lets_transform
+                                          (fun (p2 : Erasure.pcuic_program)
+                                             (H : 
+                                              Erasure.Transform.post
+                                                Erasure.template_to_pcuic_transform
+                                                p2) =>
+                                           Erasure.erasure_pipeline_obligation_1
+                                             p2 H)) p1) =>
+                              Erasure.erasure_pipeline_obligation_2 p1 H))
+                          (Erasure.remove_params_optimization
+                             EWcbvEval.default_wcbv_flags)
+                          (fun (p1 : Erasure.eprogram_env)
+                             (_ : Erasure.Transform.post
+                                    (Erasure.Transform.compose
+                                       (Erasure.Transform.compose
+                                          Erasure.template_to_pcuic_transform
+                                          Erasure.pcuic_expand_lets_transform
+                                          (fun (p2 : Erasure.pcuic_program)
+                                             (H : 
+                                              Erasure.Transform.post
+                                                Erasure.template_to_pcuic_transform
+                                                p2) =>
+                                           Erasure.erasure_pipeline_obligation_1
+                                             p2 H)) Erasure.erase_transform
+                                       (fun (p2 : Erasure.pcuic_program)
+                                          (H : Erasure.Transform.post
+                                                 (Erasure.Transform.compose
+                                                 Erasure.template_to_pcuic_transform
+                                                 Erasure.pcuic_expand_lets_transform
+                                                 (fun
+                                                 (p3 : Erasure.pcuic_program)
+                                                 (H : 
+                                                 Erasure.Transform.post
+                                                 Erasure.template_to_pcuic_transform
+                                                 p3) =>
+                                                 Erasure.erasure_pipeline_obligation_1
+                                                 p3 H)) p2) =>
+                                        Erasure.erasure_pipeline_obligation_2
+                                          p2 H)) p1) =>
+                           Erasure.erasure_pipeline_obligation_3 p1)) p0) =>
+              Erasure.erasure_pipeline_obligation_4 p0 H))
+          (Erasure.expand_program p) (todo "wf_env and welltyped term")).1
+ |})
